src/program_proof/rsm/spaxos_top.v
@@ -2,6 +2,7 @@
  * Common definitions used by every part of this project. Minimize this file.
  *)
 From Perennial.program_proof Require Export grove_prelude.
+From Perennial.program_logic Require Export atomic. (* prefer the ncfupd atomics *)
 
 Definition proposals := gmap nat string.
 Definition ballot := list bool.
